{
 "cells": [
  {
   "attachments": {},
   "cell_type": "markdown",
   "metadata": {},
   "source": [
    "# Problem 4\n",
    "\n",
    "Given $f(x) = x^4 + 2x^2 - x - 3$, and that $f(p) = 0$, then:\n",
    "\n",
    "$g_1:$\n",
    "\n",
    "\\begin{gather*}\n",
    "\n",
    "x = (3 + x - 2x^2)^{\\frac{1}{4}} \\\\ \n",
    "x^4 = 3 + x - 2x^2 \\\\ \n",
    "x^4 + 2x^2 - x - 3 = 0 \\\\\n",
    "\\text{If } f(p) = 0, \\text{ then,} \\\\ \n",
    "p^4 + 2p^2 - p - 3 = 0 \\\\\n",
    "f(p) = 0 \\checkmark\n",
    "\n",
    "\\end{gather*}\n",
    "\n",
    "$g_2:$\n",
    "\n",
    "\\begin{gather*}\n",
    "\n",
    "x = (\\frac{x + 3 - x^4}{2})^{1/2}\\\\ \n",
    "x^2 = \\frac{x + 3 - x^4}{2} \\\\ \n",
    "2x^2 = x + 3 - x^4 \\\\ \n",
    "x^4 + 2x^2 - x - 3 = 0 \\\\\n",
    "\\text{If } f(p) = 0, \\text{ then,} \\\\ \n",
    "p^4 + 2p^2 - p - 3 = 0 \\\\\n",
    "f(p) = 0 \\checkmark\n",
    "\n",
    "\\end{gather*}\n",
    "\n",
    "$g_3:$\n",
    "\n",
    "\\begin{gather*}\n",
    "\n",
    "x = (\\frac{x + 3}{x^2 + 2})^{\\frac{1}{2}} \\\\\n",
    "x^2 = \\frac{x + 3}{x^2 + 2} \\\\ \n",
    "x^4 + 2x^2 = x + 3 \\\\\n",
    "x^4 + 2x^2 - x - 3 = 0 \\\\\n",
    "\\text{If } f(p) = 0, \\text{ then,} \\\\ \n",
    "p^4 + 2p^2 - p - 3 = 0 \\\\\n",
    "f(p) = 0 \\checkmark\n",
    "\n",
    "\\end{gather*}\n",
    "\n",
    "$g_4:$\n",
    "\n",
    "\\begin{gather*}\n",
    "\n",
    "x = \\frac{3x^4 + 2x^2 + 3}{4x^3 + 4x - 1} \\\\\n",
    "4x^4 + 4x^2 - x = 3x^4 + 2x^2 + 3 \\\\ \n",
    "x^4 + 2x^2 - x - 3 = 0 \\\\\n",
    "\\text{If } f(p) = 0, \\text{ then,} \\\\ \n",
    "p^4 + 2p^2 - p - 3 = 0 \\\\\n",
    "f(p) = 0 \\checkmark\n",
    "\n",
    "\\end{gather*}\n",
    "\n",
    "<div style=”page-break-after: always;”></div>"
   ]
  }
 ],
 "metadata": {
  "language_info": {
   "name": "python"
  },
  "orig_nbformat": 4
 },
 "nbformat": 4,
 "nbformat_minor": 2
}
